The relevant principle of inclusion-exclusion states
\[
|A_1 \cup A_2| = |A_1| + |A_2| - |A_1 \cap A_2| 
\]
We are given
\begin{align*}
|A_1| &= 12 \\
|A_2| &= 18 
\end{align*}

(a)
From the principle of inclusion-exclusion, we have
\begin{align*}
|A_1 \cup A_2| = 12 + 18 - 0 = 30
\end{align*}
ANSWER:
\answerbox{30}


(b)
From the principle of inclusion-exclusion, we have
\begin{align*}
|A_1 \cup A_2| = 12 + 18 - 1 = 29
\end{align*}
ANSWER:
\answerbox{29}

(c)
From the principle of inclusion-exclusion, we have
\begin{align*}
|A_1 \cup A_2| = 12 + 18 - 6 = 24
\end{align*}
ANSWER:
\answerbox{24}

(d) Since $A_1\subseteq A_2$, we have $A_1 \cap A_2 = A_1$.
Therefore
from the principle of inclusion-exclusion, we have
\begin{align*}
|A_1 \cup A_2| = |A_1| + |A_2| - |A_1 \cap A_2| = |A_1| + |A_2| - |A_1| = 
|A_2| = 18
\end{align*}
ANSWER:
\answerbox{18}

\qed
