
The characteristic equation of 
$a_n = 6 a_{n - 1} - 12 a_{n - 1} + 8 a_{n - 3} + F(n)$
is
\[
x^3 - 6 x^2 + 12 x - 8
\]
By trial and error, $2$ is a root.
By long division
\[
x^3 - 6 x^2 + 12 x - 8 = (x - 2)(x^2 - 4x + 4)
\]
Hence
\[
x^3 - 6 x^2 + 12 x - 8 = (x - 2)^3
\]
Hence the roots of $x^3 - 6 x^2 + 12 x - 8$ are $r_1 = r_2 = r_3 = 2$.
Therefore the general solution to homogeneous part of the
recurrence relation is
\[
a^{(h)}_n = C_1 2^n + C_2 2^n + C_1 n^2 2^n 
\]

(a)
The general form of
the closed form for $a_n = 6 a_{n - 1} - 12 a_{n - 1} + 8 a_{n - 3} + n^2$
is
\[
a_n = C_1 2^n + C_2 2^n + C_1 n^2 2^n + A + Bn + Cn^2
\]


(b)
The general form of
the closed form for $a_n = 6 a_{n - 1} - 12 a_{n - 1} + 8 a_{n - 3} + 2^n$
is
\[
a_n = C_1 2^n + C_2 n2^n + C_1 n^2 2^n + An^3 2^n
\]


(c)
The general form of
the closed form for $a_n = 6 a_{n - 1} - 12 a_{n - 1} + 8 a_{n - 3} + n2^n$
is
\[
a_n = C_1 2^n + C_2 n2^n + C_3 n^2 2^n + (A + Bn)n^3 2^n
\]
where $C_1, C_2, C_3, A, B$ are constants.


(d)
The general form of
the closed form for $a_n = 6 a_{n - 1} - 12 a_{n - 1} + 8 a_{n - 3} + (-2)^n$
is
\[
a_n = C_1 2^n + C_2 n2^n + C_3 n^2 2^n + A(-2)^n
\]
where $C_1, C_2, C_3, A$ are constants.


(e)
The general form of
the closed form for $a_n = 6 a_{n - 1} - 12 a_{n - 1} + 8 a_{n - 3} + n^2 2^n$
is
\[
a_n = C_1 2^n + C_2 n2^n + C_3 n^2 2^n + (A + Bn + Cn^2) n^3 2^n
\]
where $C_1, C_2, C_3, A, B, C$ are constants.


(f)
The general form of
the closed form for $a_n = 6 a_{n - 1} - 12 a_{n - 1} + 8 a_{n - 3} + n^3 (-2)^n$
is
\[
a_n = C_1 2^n + C_2 n2^n + C_3 n^2 2^n + (A + Bn + Cn^2 + Dn^3)(-2)^n
\]
where $C_1, C_2, C_3, A, B, C, D$ are constants.


(g)
The general form of
the closed form for $a_n = 6 a_{n - 1} - 12 a_{n - 1} + 8 a_{n - 3} + 3$
is
\[
a_n = C_1 2^n + C_2 n2^n + C_3 n^2 2^n + A
\]
where $C_1, C_2, C_3, A$ are constants.
