
(a)
The characteristic equation of
\[
a_n = 
\begin{cases}
  2 a_{n-1}  &\text{for $n \geq 1$} \\
  3         &\text{for $n \geq 0$}
\end{cases}
\]
is
\[
x - 2
\]
The root is $r_1 = 2$.
Therefore the general closed form for $a_n$ is
\[
a_n = C_1 2^n
\]
From the base condition
\[
3 = C_1 2^0 = C_1
\]
Hence
\[
a_n = 3 \cdot 2^n = 3^{n + 1}
\]
for $n \geq 0$.
\qed

(Check: $a_0 = 3, a_1 = 3 \cdot 2^1 = 6 = 2 \cdot 3 = 2 \cdot a_0, a_2 = 3 \cdot 2^2 = 12 = 2 \cdot 6 = 2 \cdot a_1$, $a_3 = 3 \cdot 2^3 = 24 = 2 \cdot 12 = 2 \cdot a_2$.)


(b)
The characteristic equation of
\[
a_n = 
\begin{cases}
  a_{n-1}  &\text{if } n \geq 1 \\
  2       &\text{if } n = 0
\end{cases}
\]
is
\[
x - 1
\]
The root is $r_1 = 1$.
Therefore the general closed form for $a_n$ is
\[
a_n = C_1 1^n = C_1
\]
From the base condition
\[
2 = a_0 = C_1
\]
Hence
\[
a_n = 2 
\]
for $n \geq 0$.
\qed

(Check: $a_0 = 2, a_1 = 2 = a_0, a_2 = 2 = a_1$, $a_3 = 2 = a_2$.)


(c)
The characteristic equation of
\[
a_n = 
\begin{cases}
  5 a_{n-1} - 6 a_{n-2} &\text{if } n \geq 2 \\
  1                   &\text{if } n = 0  \\
  0                   &\text{if } n = 1 
\end{cases}
\]
is
\[
x^2 - 5x + 6
\]
The roots are $r_1 = 2$, $r_2 = 3$.
Therefore the general closed form for $a_n$ is
\[
a_n = C_1 2^n + C_2 3^n
\]
From the base cases
\begin{align*}
1 &= a_0 = C_1 + C_2 \\
0 &= a_1 = 2C_1 + 3C_2 \\
\end{align*}
Therefore $C_1 = 3, C_2 = -2$
Hence
\[
a_n = 3 \cdot 2^n - 2 \cdot 3^n
\]
for $n \geq 0$.
\qed

(Check:
\begin{console}[fontsize=\footnotesize]
def an(n):
    if n == 0: return 1
    elif n == 1: return 0
    else: return 5 * an(n - 1) - 6 * an(n - 2)

def bn(n):
    return 3 * 2**n - 2 * 3**n

for n in range(10):
    print(n, an(n), bn(n))
\end{console}
has output
\begin{console}[fontsize=\footnotesize]
0 1 1
1 0 0
2 -6 -6
3 -30 -30
4 -114 -114
5 -390 -390
6 -1266 -1266
7 -3990 -3990
8 -12354 -12354
9 -37830 -37830
\end{console}
)


(d)
The characteristic equation of
\[
a_n = 
\begin{cases}
  4 a_{n-1} - 4 a_{n-2} &\text{if } n \geq 2 \\
  6                   &\text{if } n \geq 0 \\
  8                   &\text{if } n \geq 1
\end{cases}
\]
is
\[
x^2 - 4x + 4
\]
The roots are $r_1 = 2$, $r_2 = 2$.
Therefore the general closed form for $a_n$ is
\[
a_n = C_1 2^n + C_2 n2^n
\]
From the base cases
\begin{align*}
6 &= a_0 = C_1 \\
8 &= a_1 = 2C_1 + 2C_2 \\
\end{align*}
Therefore $C_1 = 6, C_2 = -2$
Hence
\[
a_n = 6 \cdot 2^n - 2 \cdot n 2^n = (6 - 2n) 2^n
\]
for $n \geq 0$.
\qed

Check:
\begin{console}[fontsize=\footnotesize]
def an(n):
    if n == 0: return 6
    elif n == 1: return 8
    else: return 4 * an(n-1) - 4 * an(n - 2)

def bn(n):
    return 6 * 2**n - 2 * n * 2**n

for n in range(10):
    print(n, an(n), bn(n))
\end{console}
\begin{console}[fontsize=\footnotesize]
0 6 6
1 8 8
2 8 8
3 0 0
4 -32 -32
5 -128 -128
6 -384 -384
7 -1024 -1024
8 -2560 -2560
9 -6144 -6144
\end{console}


(e)
The characteristic equation of
\[
a_n = 
\begin{cases}
 - 4 a_{n-1} - 4 a_{n-2} &\text{if } n \geq 2 \\
  0                    &\text{if } n = 0 \\
  1                    &\text{if } n = 1
\end{cases}
\]
is
\[
x^2 + 4x + 4
\]
The roots are $r_1 = -2$, $r_2 = -2$.
Therefore the general closed form for $a_n$ is
\[
a_n = C_1 (-2)^n + C_2 n(-2)^n
= C_1 (-1)^n 2^n + C_2 n(-1)^n 2^n
= (C_1 + C_2 n) (-1)^n 2^n
\]
From the base cases
\begin{align*}
0 &= a_0 = C_1 \\
1 &= a_1 = -2C_1 - 2C_2 
\end{align*}
Therefore $C_1 = 0, C_2 = -1/2$
Hence
\[
a_n = (0 + (-1/2)n) (-1)^n 2^n = (-1)^{n+1} n 2^{n - 1}
\]
for $n \geq 0$.
\qed

Check:
\begin{console}[fontsize=\footnotesize]
def an(n):
    if n == 0: return 0
    elif n == 1: return 1
    else: return -4 * an(n - 1) - 4 * an(n - 2)

def bn(n):
    return (-1)**(n + 1) * n * 2**(n - 1)

for n in range(10):
    print(n, an(n), bn(n))
\end{console}
\begin{console}[fontsize=\footnotesize]
0 0 0.0
1 1 1
2 -4 -4
3 12 12
4 -32 -32
5 80 80
6 -192 -192
7 448 448
8 -1024 -1024
9 2304 2304
\end{console}


(f)
The characteristic equation of
\[
a_n = 
\begin{cases}
  4 a_{n-2} &\text{if } n \geq 2 \\
  0        &\text{if } n = 0 \\
  4        &\text{if } n = 1
\end{cases}
\]
is
\[
x^2 - 4
\]
The roots are $r_1 = -2$, $r_2 = 2$.
Therefore the general closed form for $a_n$ is
\[
a_n = C_1 (-2)^n + C_2 2^n
= C_1 (-1)^n 2^n + C_2 2^n
= ((-1)^n C_1 + C_2) 2^n
\]
From the base cases
\begin{align*}
0 &= a_0 = C_1 + C_2 \\
4 &= a_1 = -2C_1 + 2C_2 
\end{align*}
Therefore $C_1 = -1, C_2 = 1$
Hence
\[
a_n = ((-1)^n (-1) + 1) 2^n = ((-1)^{n+1} + 1) 2^n
\]
for $n \geq 0$.
\qed

Check:
\begin{console}[fontsize=\footnotesize]
def an(n):
    if n == 0: return 0
    elif n == 1: return 4
    else: return  4 * an(n - 2)

def bn(n):
    return ((-1)**(n+1) + 1) * 2**n

for n in range(10):
    print(n, an(n), bn(n))
\end{console}
\begin{console}[fontsize=\footnotesize]
0 0 0
1 4 4
2 0 0
3 16 16
4 0 0
5 64 64
6 0 0
7 256 256
8 0 0
9 1024 1024
\end{console}


(g)
The characteristic equation of
\[
a_n = 
\begin{cases}
  a_{n-2}/4 &\text{if } n \geq 2 \\
  1        &\text{if } n = 0 \\
  0        &\text{if } n = 1
\end{cases}
\]
is
\[
x^2 - 1/4
\]
The roots are $r_1 = -1/2$, $r_2 = 1/2$.
Therefore the general closed form for $a_n$ is
\[
a_n = C_1 (-1/2)^n + C_2 (1/2)^n
= C_1 (-1)^n (1/2)^n + C_2 (1/2)^n
= ((-1)^n C_1 + C_2) (1/2)^n
\]
From the base cases
\begin{align*}
1 &= a_0 = C_1 + C_2 \\
0 &= a_1 = -C_1 + C_2 
\end{align*}
Therefore $C_1 = 1/2, C_2 = 1/2$
Hence
\[
a_n = ((-1)^n (1/2) + (1/2)) (1/2)^n = ((-1)^{n} + 1) (1/2)^{n + 1}
\]
for $n \geq 0$.
\qed

Check:
\begin{console}[fontsize=\footnotesize]
def an(n):
    if n == 0: return 1
    elif n == 1: return 0
    else: return  an(n - 2) / 4.0

def bn(n):
    return ((-1)**n + 1) * 0.5**(n + 1)

for n in range(10):
    print(n, an(n), bn(n))
\end{console}
\begin{console}[fontsize=\footnotesize]
0 1 1.0
1 0 0.0
2 0.25 0.25
3 0.0 0.0
4 0.0625 0.0625
5 0.0 0.0
6 0.015625 0.015625
7 0.0 0.0
8 0.00390625 0.00390625
9 0.0 0.0
\end{console}


