\input{thispreamble.tex}

\renewcommand\AUTHOR{jdoe5@cougars.ccis.edu} % CHANGE TO YOURS

\begin{document}
\topmattertwo

\textsc{Objectives}
\begin{enumerate}[nosep]
\item Use generating functions to compute closed forms for linear recurrences.
\item Use generating functions to compute/prove identities.
\item Use characteristic equation to compute closed forms for
linear recurrences.
\end{enumerate}
\vspace{1cm}



The following are practice problems for self-study:
\begin{enumerate}[nosep]
\li Rosen 8th edition, section 8.2: Odd numbered problems 1-53 except 41,49,51.
\end{enumerate}
For this assignment the problems you need to solve are
\begin{enumerate}[nosep]
\li Q1 and Q2 and 
\li Rosen 8th edition, section 8.2:
\underline{questions 4, 12, 28, 30}.
\end{enumerate}
Explain your work completely using the solutions provided as
guide and examples on how to write math properly.

In \LaTeX\, math notation is enclosed by the \verb!$! symbols.
For instance \verb!$x = a_{1} + b^{2}$! gives you $x = a_{1} + b^{2}$.
For emphasis you can write also write it as
\verb!\[ x = a_{1} + b^{2} \]!
to center your math:
\[
x = a_{1} + b^{2}
\]
For binomial coefficients, \verb!$\binom{5}{2}$! will give you 
$\binom{5}{2}$.

If you are writing a series of computations you can align them like this:
\begin{Verbatim}[frame=single,fontsize=\footnotesize]
\begin{align*}
a(x) &= \sum_{n=0}^\infty a_n x^n \\
     &= a_0 + a_1 x + \sum_{n=2}^\infty a_n x^n \\
     &= 123 + 234 x + \sum_{n=2}^\infty (a_{n-1} + 1) x^n \\
\end{align*}
\end{Verbatim}
gives you this:
\begin{align*}
a(x) &= \sum_{n=0}^\infty a_n x^n \\
     &= a_0 + a_1 x + \sum_{n=2}^\infty a_n x^n \\
     &= 123 + 234 x + \sum_{n=2}^\infty (a_{n-1} + 1) x^n \\
\end{align*}

For more information about \LaTeX\, go to my
website
\href{http://bit.ly/yliow0}{http://bit.ly/yliow0},
click on \verb!Yes!
you are one of my students,
then look for
\href{https://drive.google.com/file/d/0BzjYrK0VFuMWZm5xV0kyR3J2Zm8/view?usp=sharing}{latex.pdf}.)
Even easier: ask questions in CCCS discord.

Draw a box around your final answer if the question required
an explicit answer (i.e., if it's not a proof question).

\newpage
\input{solving-linear-recurrences.tex}

%------------------------------------------------------------------------------
\newpage
\nextq Find a closed form for $0^3 + 1^3 + 2^3 + \cdots + n^3$.

\SOLUTION

\input{sum-of-cubes.tex}

%------------------------------------------------------------------------------
\newpage
\nextq
Using generating function method, find a closed form for $a_n$ where
\[
a_n = 5a_{n-1} - 6a_{n-2} + \underline{3n + 1}
\]
where $a_0 = 2$ and $a_1 = 3$.

\SOLUTION

\input{gen-func-nonhomogeneous.tex}

%------------------------------------------------------------------------------
\newpage
\nextq Rosen 8th edition, section 8.2, question 1.

\SOLUTION

\input{08-02-01.tex}

%------------------------------------------------------------------------------
\newpage
\nextq Rosen 8th edition, section 8.2, question 3.

\SOLUTION

\input{08-02-03.tex}

%------------------------------------------------------------------------------
\newpage
\nextq Rosen 8th edition, section 8.2, question 4.

\SOLUTION
Solve these recurrence relations together with the initial
conditions given.

a)

$r^2 -r -6 = 0$

$r=-2,3$

$a_n = a_1(-2)^n + a_23^n$

$3 = a_1 + a_2$

$6= -2a_1 + 3a_2$

$a_1 = \frac{3}{5}$ $a_2 = \frac{12}{5}$

$a_n = (\frac{3}{5})(-2)^n + (\frac{12}{5})3^n$

b)

$r^2 - 6r +10 = 0$

$r=-2,5$

$a_n = a_12^n + a_25^n$

$2 = a_1 + a_2$

$1= -2a_1 + 5a_2$

$a_1 = 3$ $a_2 = -1$

$a_n = 3 \cdot 2^n - 5^n$

c) 

$r^2 - 6r +8 = 0$

$r=-2,4$

$a_n = a_12^n + a_24^n$

$4 = a_1 + a_2$

$10= -2a_1 + 4a_2$

$a_1 = 3$ $a_2 = 1$

$a_n = 3 \cdot 2^n - 4^n$

d) 

$r^2 - 2r +1 = 0$

$r=-1,1$

$a_n = a_11^n + a_21^n$

$4 = a_1 $

$1= a_1 + a_2$

$a_1 = 4$ $a_2 = -3$

$a_n = 4  - 3^n$

e)

$r^2 - 1 = 0$

$r=-1,1$

$a_n = a_1(-1)^n + a_21^n$

$5 = a_1 + a_2$

$-1= -a_1 + a_2$

$a_1 = 3$ $a_2 = 2$

$a_n = 3 \cdot (-1)^n +2$

(f)

$r^2 + 6r + 9 = 0$

$r=-3,-3$

$a_n = a_1(-3)^n + a_2(-3)^n$

$3 = a_1$

$-3= -3a_1 +-3a_2$

$a_1 = 3$ $a_2 = -2$

$a_n = 3(-3)^n - 2n(-3)^n$

(g)

$r^2 +4r -5 = 0$

$r=-5,1$

$a_n = a_1(-5)^n + a_21^n$

$2 = a_1 + a_2$

$8= -5a_1 + a_2$

$a_1 = -1$ $a_2 = 3$

$a_n = -(-5)^n + 3$







\input{08-02-04.tex}

%------------------------------------------------------------------------------
\newpage
\nextq Rosen 8th edition, section 8.2, question 12.

\SOLUTION

$r^3 -2r^2 - r + 2 =0$

$r = 1,-1,2$

$a_n = a_1 + a_2(-1)^n + a_32^n $

$3 = a_1 + a_2 + a_3$

$ 6 = a_1 - a_2 + 2a_3$

$ a-1 = 6, a_2 = -2, a_3 = -1$

$a_n = 6 - 2(-1)^n - 2^n$



\input{08-02-12.tex}

%------------------------------------------------------------------------------
\newpage
\nextq Rosen 8th edition, section 8.2, question 13.

\SOLUTION

\input{08-02-13.tex}

%------------------------------------------------------------------------------
\newpage
\nextq Rosen 8th edition, section 8.2, question 23.

\SOLUTION

\input{08-02-23.tex}

%------------------------------------------------------------------------------
\newpage
\nextq Rosen 8th edition, section 8.2, question 24.

\SOLUTION

\input{08-02-24.tex}

%------------------------------------------------------------------------------
\newpage
\nextq Rosen 8th edition, section 8.2, question 25.

\SOLUTION

\input{08-02-25.tex}

%------------------------------------------------------------------------------
\newpage
\nextq Rosen 8th edition, section 8.2, question 25.

\SOLUTION

\input{08-02-25.tex}

%------------------------------------------------------------------------------
\newpage
\nextq Rosen 8th edition, section 8.2, question 26.

\SOLUTION

\input{08-02-26.tex}

%------------------------------------------------------------------------------
\newpage
\nextq Rosen 8th edition, section 8.2, question 28.

\SOLUTION

a)

$a_n = 2a_{n-1}$

$a_n^{(h)} = a2^n$

$p_2 = -2, 4p_2 = p_1$

$-2p_2 + 2p_1 - p_0 = 0$

$p = -8$ $p_0 = -12$

$a_n = a2^n -2n^2 -8n - 12$

b) 

$a=13$ 

$a_n = 13 \cdot 2^n - 8n - 12$
\input{08-02-28.tex}

%------------------------------------------------------------------------------
\newpage
\nextq Rosen 8th edition, section 8.2, question 30.

\SOLUTION

a)

$a_n = -5a_{n-1} - 6a_{n-2}$

$r^2 + 5r +6=0$ 

$r = -2,-3$

$a_n^{(h)} = a(-2)^n + \beta(-3)^n$

$c=16$

$a_n^{(p)} = 16 \cdot 4^n$

$a_n = a(-2)^n + \beta(-3)^n +4^{n+2}$

b)

$a_1 = 56$

$a_2 = 4a + 9 \beta + 256$

$a_n = (-2)^n + 2(-3) + 4^{n+2}$
\input{08-02-30.tex}

%------------------------------------------------------------------------------
\newpage
\input{instructions.tex}
\end{document}
