(a)
Using binomial theorem, we have
\begin{align*}
  (3x - 4)^3 &= \sum_{n=0}^3 \binom{3}{n} (3x)^n(-4)^{3 - n} \\
             &= \sum_{n=0}^3 \binom{3}{n} 3^n(-1)^{3 - n}4^{3 - n}x^n \\
             &= \sum_{n=0}^3 (-1)^{n + 1}\binom{3}{n} 4^3 \left(\frac{3}{4}\right)^n x^n 
\end{align*}
Therefore
\[
a_n =
\begin{cases}
  \binom{3}{n} (-1)^{n - 1}4^3 \left(\frac{3}{4}\right)^n & \text{if $n = 0,1,2,3$}\\
  0 & \text{otherwise}
\end{cases}
\]


(b)
Using binomial theorem, we have
\begin{align*}
(x^3 + 1)^3 &= \sum_{n=0}^3 \binom{3}{n} (x^3)^n \\
            &= \sum_{n=0}^3 \binom{3}{n} x^{3n} \\
\end{align*}
Therefore
\[
a_n =
\begin{cases}
  \binom{3}{n/3} & \text{if $n = 0, 3, 6, 9$}\\ 
  0              & \text{otherwise}
\end{cases}
\]


(c)
From
\[
  \frac{1}{1 - 5x} = \sum_{n=0}^\infty (5x)^n = \sum_{n=0}^\infty 5^n x^n
\]
we get
\[
a_n = 5^n
\]
for $n \geq 0$.


(d)
From
\begin{align*}
  \frac{x^3}{1 + 3x} &= x^3 \frac{1}{1 - (-3x)} \\
                     &= x^3 \sum_{n=0}^\infty (-3x)^n \\
                     &= x^3 \sum_{n=0}^\infty (-3)^n x^n \\
                     &= \sum_{n=0}^\infty (-3)^n x^{n+3} \\
                     &= \sum_{k=3}^\infty (-3)^{k-3} x^{k} & \text{(let $k = n + 3$)}\\
\end{align*}
we get
\[
a_n =
\begin{cases}
  0         & \text{if $n = 0, 1, 2$} \\
  (-3)^{n-3} & \text{if $n \geq 3$}
\end{cases}
\]


(e)
From
\begin{align*}
  x^2 + 3x + 7 + \frac{1}{1 - x^2}
  &= x^2 + 3x + 7 + \sum_{n=0}^\infty (x^2)^n \\
  &= x^2 + 3x + 7 + \sum_{n=0}^\infty x^{2n} \\
  &= x^2 + 3x + 7 + \left(1 + x^2 + \sum_{n=2}^\infty x^{2n} \right) \\
  &= 2x^2 + 3x + 8 + \sum_{n=2}^\infty x^{2n} 
\end{align*}
we get
\[
a_n =
\begin{cases}
  8 & \text{if $n = 0$} \\
  3 & \text{if $n = 1$} \\
  2 & \text{if $n = 2$} \\
  1 & \text{if $n \geq 4$ is even} \\
  0 & \text{if $n \geq 3$ is odd} \\
\end{cases}
\]


(f)
From
\begin{align*}
  \frac{x^4}{1 - x^4} - x^3 - x^2 - x - 1
  &= x^4 \frac{1}{1 - x^4} - x^3 - x^2 - x - 1 \\
  &= x^4 \sum_{n=0}^\infty (x^4)^n - x^3 - x^2 - x - 1 \\
  &= x^4 \sum_{n=0}^\infty x^{4n} - x^3 - x^2 - x - 1 \\
  &= \sum_{n=0}^\infty x^{4(n + 1)} - x^3 - x^2 - x - 1 \\
\end{align*}
we get
\[
a_n =
\begin{cases}
  -1 & \text{if $n = 0,1,2,3$} \\
  1 & \text{if $n = 4k$ for $k\geq 1$} \\
  0 & \text{otherwise}
\end{cases}
\]

(g)
From
\begin{align*}
  \frac{x^2}{(1 - x)^2} &= x^2 \frac{1}{(1 - x)^2} \\
  &= x^2 \sum_{n=0}^\infty \binom{2 + n - 1}{n} x^n \\
  &= x^2 \sum_{n=0}^\infty \binom{n + 1}{n} x^n \\
  &= x^2 \sum_{n=0}^\infty \binom{n + 1}{(n + 1) - n} x^n \\
  &= x^2 \sum_{n=0}^\infty \binom{n + 1}{1} x^n \\
  &= x^2 \sum_{n=0}^\infty (n + 1) x^n \\
  &= \sum_{n=0}^\infty (n + 1) x^{n+2} \\
  &= \sum_{k=2}^\infty (k - 1) x^{k} & \text{(let $k = n + 2$)}
\end{align*}
we get
\[
a_n
\begin{cases}
  0 & \text{if } n = 0,1 \\
  n-1 & \text{if } n \geq 2 
\end{cases}
\]


(g)
From
\begin{align*}
  2e^{2x} &= 2 \sum_{n=0}^\infty \frac{1}{n!} x^n \\
         &= \sum_{n=0}^\infty \frac{2}{n!} x^n 
\end{align*}
we get
\[
a_n = \frac{2}{n!}
\]
for $n \geq 0$.
