
(a)
The generating function is
\begin{align*}
  f(x) &= \sum_{i=0}^\infty (-1)x^i \\
  &= - \sum_{i=0}^\infty x^i \\
  &= - \frac{1}{1 - x} \\
  &= \frac{1}{x - 1} 
\end{align*}

(b)
The generating function is
\begin{align*}
  f(x) &= \sum_{n=1}^\infty 2^nx^n \\
  &= \sum_{n=0}^\infty (2x)^n \\
  &= \frac{1}{1 - 2x} 
\end{align*}

(c)
The generating function is
\begin{align*}
  f(x) &= \sum_{n=0}^\infty (n-1)x^n \\
  &= \sum_{n=0}^\infty nx^n - \sum_{n=0}^\infty x^n \\
  &= \sum_{n=1}^\infty nx^{n} - \frac{1}{1 - x} \\
  &= x\sum_{n=1}^\infty nx^{n-1} - \frac{1}{1 - x} \\
  &= x \sum_{n=1}^\infty \frac{d}{dx} x^{n} - \frac{1}{1 - x} \\
  &= x \frac{d}{dx} \sum_{n=1}^\infty x^{n} - \frac{1}{1 - x} \\
  &= x \frac{d}{dx} \frac{1}{1 - x} - \frac{1}{1 - x} \\
  &= x \frac{-1}{(1 - x)^2} - \frac{1}{1 - x} \\
  &= \frac{-x - (1 - x)}{(1 - x)^2}  \\
  &= -\frac{1}{(1 - x)^2}  
\end{align*}


(d)
The generating function is
\begin{align*}
  f(x) &= \sum_{n=0}^\infty \frac{1}{(n+1)!} x^n \\
  &= \frac{1}{x}\sum_{n=0}^\infty \frac{1}{(n+1)!} x^{n+1} \\
  &= \frac{1}{x}\sum_{k=1}^\infty \frac{1}{k!} x^{k} & & \text{(let $k = n + 1$)}\\
  &= \frac{1}{x}
  \left(
  \sum_{k=0}^\infty \frac{1}{k!} x^{k} - 1
  \right)\\
  &= \frac{1}{x}
  \left(
  e^x - 1
  \right)\\
  &= \frac{e^x - 1}{x}
\end{align*}
